Value analysis: take types of function parameters into account
We know that the values of function parameters match the types declared
in the function signature.  We can use this information to give more
precise initial abstract values for parameters of small integer types.

As an exception: if a parameter needs normalization on function entry
(as per the ABI), ignore its type, otherwise the normalization code
could be optimized away.

backend/ValueDomain.v
@@ -15,6 +15,7 @@ Require Import Zwf Coqlib Maps Zbits Integers Floats Lattice.
 Require Import Compopts AST.
 Require Import Values Memory Globalenvs Builtins Events.
 Require Import Registers RTL.
+Require Conventions1.
 
 (** The abstract domains for value analysis *)
 
@@ -3140,6 +3141,31 @@ Proof.
   intros v a E; destruct v; simpl in E; inv E; constructor.
 Qed.
 
+(** Lifting an extended type to a value approximation. *)
+
+Definition of_xtype (r: rettype) (p: aptr) : aval :=
+  match r with
+  | Tbool => Uns p 1
+  | Tint8signed => Sgn p 8
+  | Tint8unsigned => Uns p 8
+  | Tint16signed => Sgn p 16
+  | Tint16unsigned => Uns p 16
+  | _ => Ifptr p
+  end.
+
+Lemma of_xtype_arg_sound: forall v r p,
+  Val.has_argtype v r ->
+  vmatch v (Ifptr p) ->
+  vmatch v (of_xtype r p).
+Proof.
+  intros. destruct r, v; simpl in *; try contradiction; auto with va.
+- constructor. lia. apply is_uns_zero_ext. destruct H; subst i; auto.
+- constructor. lia. apply is_sgn_sign_ext. lia. auto.
+- constructor. lia. apply is_uns_zero_ext. auto.
+- constructor. lia. apply is_sgn_sign_ext. lia. auto.
+- constructor. lia. apply is_uns_zero_ext. auto.
+Qed.
+
 (** * Abstracting memory blocks *)
 
 Inductive acontent : Type :=
@@ -4588,36 +4614,47 @@ Proof.
   unfold AVal.eq; red; intros. subst av. inv H0.
 Qed.
 
-Fixpoint einit_regs (rl: list reg) : aenv :=
-  match rl with
-  | r1 :: rs => AE.set r1 (Ifptr Nonstack) (einit_regs rs)
-  | nil => AE.top
+Fixpoint einit_regs (rl: list reg) (tl: list rettype) : aenv :=
+  match rl, tl with
+  | nil, _ => AE.top
+  | r1 :: rs, t1 :: ts =>
+      let a1 :=
+        if Conventions1.parameter_needs_normalization t1
+        then Ifptr Nonstack
+        else of_xtype t1 Nonstack in
+      AE.set r1 a1 (einit_regs rs ts)
+  | r1 :: rs, nil => AE.set r1 (Ifptr Nonstack) (einit_regs rs nil)
   end.
 
 Lemma ematch_init:
-  forall rl vl,
+  forall rl vl tl,
+  Val.has_argtype_list vl tl ->
   (forall v, In v vl -> vmatch bc v (Ifptr Nonstack)) ->
-  ematch (init_regs vl rl) (einit_regs rl).
+  ematch (init_regs vl rl) (einit_regs rl tl).
 Proof.
-  induction rl; simpl; intros.
-- red; intros. rewrite Regmap.gi. simpl.
-  constructor.
-- destruct vl as [ | v1 vs ].
-  + assert (ematch (init_regs nil rl) (einit_regs rl)).
-    { apply IHrl. simpl; tauto. }
-    replace (init_regs nil rl) with (Regmap.init Vundef) in H0 by (destruct rl; auto).
-    red; intros. rewrite AE.gsspec. destruct (peq r a).
-    rewrite Regmap.gi. constructor.
-    apply H0.
-    red; intros EQ; rewrite EQ in H0. specialize (H0 xH). simpl in H0. inv H0.
-    unfold AVal.eq, AVal.bot. congruence.
-  + assert (ematch (init_regs vs rl) (einit_regs rl)).
-    { apply IHrl. eauto with coqlib. }
-    red; intros. rewrite Regmap.gsspec. rewrite AE.gsspec. destruct (peq r a).
-    auto with coqlib.
-    apply H0.
-    red; intros EQ; rewrite EQ in H0. specialize (H0 xH). simpl in H0. inv H0.
-    unfold AVal.eq, AVal.bot. congruence.
+Local Opaque Conventions1.parameter_needs_normalization.
+  assert (A: forall rs ae, ematch rs ae -> ae <> AE.Bot).
+  { intros; red; intros EQ. rewrite EQ in H. specialize (H 1%positive). simpl in H. inv H. }
+  assert (B: ~AVal.eq (Ifptr Nonstack) AVal.bot) by (unfold AVal.eq, AVal.bot; congruence).
+  assert (C: forall t, ~AVal.eq (of_xtype t Nonstack) AVal.bot).
+  { intros. unfold AVal.eq, AVal.bot; destruct t; simpl; congruence. }
+  induction rl; simpl; intros vl tl T V.
+- red; intros. rewrite Regmap.gi. simpl. constructor.
+- inv T.
+  + assert (REC: ematch (init_regs nil rl) (einit_regs rl nil)).
+    { apply IHrl. constructor. auto. }
+    replace (init_regs nil rl) with (Regmap.init Vundef) in REC by (destruct rl; auto).
+    red; intros. rewrite AE.gsspec by eauto. destruct (peq r a).
+    rewrite Regmap.gi; constructor.
+    apply REC.
+  + assert (REC: ematch (init_regs al rl) (einit_regs rl bl)).
+    { apply IHrl; eauto with coqlib. }
+    red; intros. rewrite Regmap.gsspec, AE.gsspec; eauto.
+    * destruct (peq r a).
+      destruct (Conventions1.parameter_needs_normalization b1);
+      auto using of_xtype_arg_sound with coqlib.
+      apply REC.
+    * destruct (Conventions1.parameter_needs_normalization b1); auto.
 Qed.
 
 Fixpoint eforget (rl: list reg) (ae: aenv) {struct rl} : aenv :=
